Rewrite sketch

Logic/Modal/Normal/Completeness.lean
@@ -6,372 +6,283 @@ import Logic.Modal.Normal.Soundness
 
 namespace LO.Modal.Normal
 
+open Finset
 open Formula Context Deduction
 
-variable {α β : Type u}
+variable {α β : Type u} [DecidableEq β]
+
+namespace Formula
+
+/-
+@[simp] def FrameConsequence (f : Frame α) (Γ : Context β) (p : Formula β) := ∀ V w, (w ⊧ᴹˢ[⟨f, V⟩] Γ) → (w ⊧ᴹˢ[⟨f, V⟩] p)
+
+notation Γ " ⊨ᴹᶠ[" f "] " p => Formula.FrameConsequence f Γ p
+notation Γ " ⊭ᴹᶠ[" f "] " p => ¬(Γ ⊨ᴹᶠ[f] p)
+
+namespace FrameConsequence
+
+variable {f : Frame α} {Γ Γ' : Context β} {p q : Formula β}
+
+@[simp] lemma def_emptyctx : (∅ ⊨ᴹᶠ[f] p) ↔ (⊧ᴹᶠ[f] p) := by aesop;
+@[simp] lemma axiomK : (Γ ⊨ᴹᶠ[f] AxiomK p q) := by aesop;
+@[simp] lemma weakening : (Γ ⊆ Γ') → (Γ ⊨ᴹᶠ[f] p) → (Γ' ⊨ᴹᶠ[f] p) := by aesop;
+@[simp] lemma modus_ponens : (Γ ⊨ᴹᶠ[f] p ⟶ q) → (Γ ⊨ᴹᶠ[f] p) → (Γ ⊨ᴹᶠ[f] q) := by aesop;
+
+end FrameConsequence
+-/
+
+def Consequence (α) (Λ : AxiomSet β) (Γ : Context β) (p : Formula β) := ∀ f ∈ FrameClass α β Λ, ∀ V w, (w ⊧ᴹˢ[⟨f, V⟩] Γ) → (w ⊧ᴹˢ[⟨f, V⟩] p)
+
+notation Γ " ⊨ᴹ[" Λ "," α "] " p => Consequence α Λ Γ p
+notation Γ " ⊭ᴹ[" Λ "," α "] " p => ¬(Γ ⊨ᴹ[Λ, α] p)
+
+end Formula
 
 section
 
-variable (α : Type u) (Λ : Logic β) (Γ : Context β)
+variable (Λ : AxiomSet β) (Γ : Context β)
 
 def Maximal := ∀ p, p ∈ Γ ∨ ~p ∈ Γ
 
-def Inconsistent := Γ ⊢ᴹ(Λ)! ⊥
+def Inconsistent (Γ : Set (Formula β)) := ∃ (Δ : Finset (Formula β)), (↑Δ ⊆ Γ) ∧ (Δ ⊢ᴹ(Λ)! ⊥)
 
-def Consistent := ¬(Inconsistent Λ Γ)
+def Consistent (Γ : Set (Formula β)) := ¬(Inconsistent Λ Γ)
 
 def WeakCompleteness := ∀ (f : Frame α) (p : Formula β), (⊧ᴹᶠ[f] p) → (⊢ᴹ(Λ) p)
 
-def Completeness := ∀ f ∈ FrameClass α β Λ, ∀ Γ (p : Formula β), (Γ ⊨ᴹᶠ[f] p) → (Γ ⊢ᴹ(Λ) p)
+def Completeness (Λ α) := ∀ Γ (p : Formula β), (Γ ⊨ᴹ[Λ, α] p) → (∃ (Δ : Finset (Formula β)), (↑Δ ⊆ Γ) → (Δ ⊢ᴹ(Λ)! p))
 
-def FrameClassSatisfiable := ∃ f ∈ FrameClass α β Λ, ∃ V w, w ⊧ᴹˢ[⟨f, V⟩] Γ
+def FrameClassSatisfiable (Λ α) (Γ : Context β) := ∃ f ∈ FrameClass α β Λ, ∃ V w, w ⊧ᴹˢ[⟨f, V⟩] Γ
 
 end
+
+variable {Λ : AxiomSet β}
+variable {Γ : Set (Formula β)} (hConsisΓ : Consistent Λ Γ)
 
 @[simp]
 lemma inconsistent_insert_falsum : Inconsistent Λ (insert ⊥ Γ) := by
   simp [Inconsistent];
-  exact ⟨axm (by simp)⟩;
-
-lemma consistent_no_falsum (hConsisΓ : Consistent Λ Γ) : ⊥ ∉ Γ := by
-  intro h;
-  have h₁ : Γ ⊢ᴹ(Λ) ⊥ := axm h;
-  have h₂ : IsEmpty (Γ ⊢ᴹ(Λ) ⊥) := by simpa [Consistent, Inconsistent] using hConsisΓ;
-  exact h₂.false h₁;
-
-lemma consistent_neither_provable (hConsisΓ : Consistent Λ Γ) : ¬((Γ ⊢ᴹ(Λ)! p) ∧ (Γ ⊢ᴹ(Λ)! ~p)) := by
-  by_contra hC;
-  exact hConsisΓ ⟨modus_ponens hC.2.some hC.1.some⟩;
+  existsi {⊥};
+  exact ⟨(by simp), ⟨axm (by simp)⟩⟩;
 
 @[simp]
-lemma consistent_neg_undeducible (hConsisΓ : Consistent Λ Γ) : (Γ ⊢ᴹ(Λ)! p) → (Γ ⊬ᴹ(Λ)! ~p) := fun h hc => consistent_neither_provable hConsisΓ ⟨h, hc⟩
+lemma consistent_isempty_falsum (Δ : Finset (Formula β)) (hΔ : ↑Δ ⊆ Γ) : IsEmpty (Δ ⊢ᴹ(Λ) ⊥) := by
+  simp [Inconsistent, Consistent] at hConsisΓ;
+  exact hConsisΓ Δ (by assumption);
 
-lemma consistent_neither_included (hConsisΓ : Consistent Λ Γ) : ¬(p ∈ Γ ∧ ~p ∈ Γ) := by
+lemma consistent_no_falsum : ∀ (Δ : Finset (Formula β)), ↑Δ ⊆ Γ → ⊥ ∉ Δ := by
+  intro Δ hΔ;
   by_contra hC;
-  exact consistent_neither_provable hConsisΓ ⟨⟨axm hC.1⟩, ⟨axm hC.2⟩⟩;
+  have h₁ : Δ ⊢ᴹ(Λ) ⊥ := axm hC;
+  have h₂ : IsEmpty (Δ ⊢ᴹ(Λ) ⊥) := consistent_isempty_falsum hConsisΓ Δ hΔ;
+  exact h₂.false h₁;
 
-lemma consistent_subset {Γ Δ : Context β} : (Γ ⊆ Δ) → (Consistent Λ Δ) → (Consistent Λ Γ) := by
-  intro hs _ hInconsisΓ;
-  suffices Δ ⊢ᴹ(Λ)! ⊥ by aesop;
-  exact ⟨weakening' _ hs hInconsisΓ.some⟩;
+lemma consistent_no_falsum' : ⊥ ∉ Γ := by
+  by_contra;
+  apply consistent_no_falsum hConsisΓ {⊥} (by aesop);
+  simp;
+
+lemma consistent_neither_provable : ∀ (Δ : Finset (Formula β)), ↑Δ ⊆ Γ → ¬((Δ ⊢ᴹ(Λ)! p) ∧ (Δ ⊢ᴹ(Λ)! ~p)) := by
+  intro Δ hΔ;
+  by_contra hC;
+  have := consistent_isempty_falsum hConsisΓ Δ hΔ;
+  exact this.false (modus_ponens hC.2.some hC.1.some);
+
+lemma consistent_neg_undeducible : ∀ (Δ : Finset (Formula β)), ↑Δ ⊆ Γ → (Δ ⊢ᴹ(Λ)! p) → (Δ ⊬ᴹ(Λ)! ~p) := by
+  intro Δ hΔ hp hn;
+  exact consistent_neither_provable hConsisΓ Δ hΔ ⟨hp, hn⟩;
+
+lemma consistent_neither_included : ∀ (Δ : Finset (Formula β)), ↑Δ ⊆ Γ → ∀ p, ¬(p ∈ Δ ∧ ~p ∈ Δ) := by
+  intro Δ hΔ p;
+  by_contra hC;
+  exact consistent_neither_provable hConsisΓ Δ hΔ ⟨⟨axm hC.1⟩, ⟨axm hC.2⟩⟩;
+
+lemma consistent_subset {Γ₁ Γ₂ : Context β} : (Γ₁ ⊆ Γ₂) → (Consistent Λ Γ₂) → (Consistent Λ Γ₁) := by
+  intro hs hConsisΓ₂ hInconsisΓ₁;
+  simp [Consistent, Inconsistent] at hConsisΓ₂ hInconsisΓ₁;
+  have ⟨Δ, hΔ₁, hΔ₂⟩ := hInconsisΓ₁;
+  exact (hConsisΓ₂ Δ (Set.Subset.trans hΔ₁ hs)).false hΔ₂.some;
 
 lemma consistent_insert {Γ : Context β} {p : Formula β} : (Consistent Λ (insert p Γ)) → (Consistent Λ Γ) := consistent_subset (by simp)
 
-lemma neg_consistent_intro_undeducible (_ : Consistent Λ (insert (~p) Γ)) : (Γ ⊬ᴹ(Λ)! p) := by
+lemma neg_consistent_intro_undeducible (hConsis : Consistent Λ (insert (~p) Γ)) : ∀ (Δ : Finset (Formula β)), ↑Δ ⊆ Γ → (Δ ⊬ᴹ(Λ)! p) := by
+  simp [Inconsistent, Consistent] at hConsis;
+  intro Δ hΔ;
   by_contra hC;
-  suffices (insert (~p) Γ ⊢ᴹ(Λ) ⊥) by have : (insert (~p) Γ ⊢ᴹ(Λ)! ⊥) := ⟨this⟩; aesop;
-  have h₁ : insert (~p) Γ ⊢ᴹ(Λ) p := Deduction.weakening' _ (by simp) hC.some;
-  have h₂ : insert (~p) Γ ⊢ᴹ(Λ) p ⟶ ⊥ := by {
-    have : insert (~p) Γ ⊢ᴹ(Λ) ~p := Deduction.axm (by simp);
+  suffices (insert (~p) Δ ⊢ᴹ(Λ) ⊥) by
+    have : insert (~p) Δ ⊢ᴹ(Λ)! ⊥ := ⟨this⟩;
+    have : insert (~p) Δ ⊬ᴹ(Λ)! ⊥ := by simpa using hConsis (insert (~p) Δ) (by simpa using Set.insert_subset_insert hΔ);
+    aesop;
+  have h₁ : insert (~p) Δ ⊢ᴹ(Λ) p := weakening' _ (by simp) hC.some;
+  have h₂ : insert (~p) Δ ⊢ᴹ(Λ) p ⟶ ⊥ := by {
+    have : insert (~p) Δ ⊢ᴹ(Λ) ~p := axm (by simp);
     simpa [Formula.neg_eq] using this;
   };
-  exact Deduction.modus_ponens h₂ h₁;
+  exact modus_ponens h₂ h₁;
 
-lemma undeducible_intro_neg_consistent (h : Γ ⊬ᴹ(Λ)! p) : (Consistent Λ (insert (~p) Γ)) := by sorry;
+lemma undeducible_intro_neg_consistent {Γ} (h : Γ ⊬ᴹ(Λ)! p) : (Consistent Λ (insert (~p) Γ)) := by
+  by_contra hC;
 
+  simp [Consistent, Inconsistent] at hC;
+  have ⟨Δ, hΔ₁, hΔ₂⟩ := hC;
+  admit;
+
+  /-
+  by_cases hp : (~p) ∈ Δ;
+  . have hΔ : Δ = insert (~p) (Δ.erase (~p)) := by aesop;
+    rw [hΔ] at hΔ₁ hΔ₂;
+    have : Γ ⊢ᴹ(Λ) p := modus_ponens (dne Γ p) (by
+      rw [neg_eq, neg];
+      have : Γ ⊢ᴹ(Λ) (~p) ⟶ ⊥ := hΔ₂.some.drop.weakening' (by
+        have := Finset.erase_subset_erase (~p) hΔ₁;
+        have := Finset.erase_ssubset_insert Γ (~p);
+      );
+
+      simpa using hC.some.drop;
+    );
+
+  have : Γ ⊢ᴹ(Λ) p := modus_ponens (dne Γ p) (by
+    rw [neg_eq, neg];
+    simpa using hC.some.drop;
+  );
+  exact h ⟨this⟩;
+  -/
+
+lemma def_not_FrameclassSatisfiable : (Γ ⊭ᴹ[Λ, α] p) ↔ (FrameClassSatisfiable Λ α (insert (~p) Γ)) := by
+  simp only [FrameClassSatisfiable, Consequence];
+  aesop;
+
+lemma intro_Completeness : (∀ (Γ : Context β), Consistent Λ Γ → FrameClassSatisfiable Λ α Γ) → (Completeness Λ α) := by
+  simp [Completeness];
+  intro h₁ Γ p h₂;
+  have := h₁ Γ;
+  sorry;
+
+  /-
+  intro h f hf Γ p hΓp;
+  suffices Γ ⊭ᴹᶠ[f] p by have := this hΓp; contradiction;
+  exact (def_not_FrameclassSatisfiable ht).mpr (h (insert (~p) Γ) (by sorry)) f hf;
+  -/
+
+/-
 lemma maximal_consistent_modus_ponens (hConsisΓ : Consistent Λ Γ) (hMaximalΓ : Maximal Γ) : (p ∈ Γ) → ((p ⟶ q) ∈ Γ) → (q ∈ Γ) := by
   intro hp hpq; by_contra hnq;
+  apply consistent_neither_provable hConsisΓ;
+  /-
   exact consistent_neither_provable hConsisΓ ⟨
     ⟨modus_ponens (axm hpq) (axm hp)⟩,
     ⟨axm (show ~q ∈ Γ from have := hMaximalΓ q; by simp_all)⟩
   ⟩;
+  -/
+-/
 
-lemma intro_Completeness : (∀ (Γ : Context β), Consistent Λ Γ → FrameClassSatisfiable α Λ Γ) → (Completeness α Λ) := by sorry;
-  -- simp [Completeness];
-  -- intro hSatisfiable f Γ p h₁ h₂;
-
-structure ConsistentTheory (Λ : Logic β) where
+structure MaximalConsistentTheory (Λ : AxiomSet β) where
   theory : Context β
   consistent : Consistent Λ theory
+  maximal : ∀ Δ, Consistent Λ Δ → theory ⊆ Δ → theory = Δ
 
-structure MaximalConsistentTheory (Λ : Logic β) where
-  theory : Context β
-  consistent : Consistent Λ theory
-  maximal : Maximal theory
+lemma mct_maximality (Ω : MaximalConsistentTheory Λ) : ∀ p, p ∈ Ω.theory ∨ ~p ∈ Ω.theory := by
+  intro p;
+  by_cases hConsis₁ : Consistent Λ (insert p Ω.theory);
+  . have h := Ω.maximal (insert p Ω.theory) hConsis₁ (by simp);
+    rw [h];
+    simp;
+  . have h := Ω.maximal (insert (~p) Ω.theory) (by
+      by_contra hConsis₂;
+      simp [Consistent, Inconsistent] at hConsis₁ hConsis₂;
+      have ⟨Δ₁, h₁₁, h₁₂⟩ := hConsis₁;
+      have ⟨Δ₂, h₂₁, h₂₂⟩ := hConsis₂;
+      have : Inconsistent Λ Ω.theory := by sorry;
+      apply Ω.consistent this;
+    ) (by simp);
+    rw [h];
+    simp;
+  -- have := Ω.maximal (insert p Ω.theory);
 
-lemma lindenbaum (Γ : Context β) (hConsisΓ : Consistent Λ Γ) :
-  ∃ (Γ' : Context β), (Consistent Λ Γ') ∧ (Maximal Γ') ∧ (Γ ⊆ Γ') := by sorry;
+lemma axiomset_include (Ω : MaximalConsistentTheory Λ) : Λ ⊆ Ω.theory := by
+  intro p hp;
+  by_contra hC;
+  have hConsis := by simpa [Consistent, Inconsistent] using Ω.consistent;
+  have : ~p ∈ Ω.theory := by simpa [hC] using mct_maximality Ω p;
+  have h₂ : {~p} ⊬ᴹ(Λ)! ⊥ := by simpa using hConsis {~p} (by aesop);
+  have h₃ : ⊢ᴹ(Λ) ~~p := by {
+    have : ⊢ᴹ(Λ) p := maxm hp;
+    admit
+  }
+  have : {~p} ⊢ᴹ(Λ) ⊥ := by simpa using h₃.dtl;
+  exact h₂ ⟨this⟩;
 
-lemma lindenbaum' (Γ : Context β) (hConsisΓ : Consistent Λ Γ) :
-  ∃ (MΓ : MaximalConsistentTheory Λ), (Γ ⊆ MΓ.theory) := by
-  have ⟨Γ', ⟨hConsisΓ', hMaximalΓ', hΓΓ'⟩⟩ := lindenbaum Γ hConsisΓ;
-  existsi ⟨Γ', hConsisΓ', hMaximalΓ'⟩; assumption;
+lemma exists_maximal_consistent_theory (hConsisΓ : Consistent Λ Γ) :
+  ∃ Γ', Consistent Λ Γ' ∧ Γ ⊆ Γ' ∧ ∀ Δ, Consistent Λ Δ → Γ' ⊆ Δ → Δ = Γ' :=
+  zorn_subset_nonempty { Γ' | Consistent Λ Γ' } (by
+    intro c hc chain hnc;
+    existsi ⋃₀ c;
+    constructor;
+    . simp;
+      by_contra hC;
+      suffices Consistent Λ (⋃₀ c) by aesop;
+      admit;
+    . apply Set.subset_sUnion_of_mem
+  ) Γ hConsisΓ
 
-def CanonicalModel (Λ : Logic β) : Model (MaximalConsistentTheory Λ) β where
+lemma lindenbaum (hConsisΓ : Consistent Λ Γ) : ∃ (Ω : MaximalConsistentTheory Λ), (Γ ⊆ Ω.theory) := by
+  have ⟨Γ', ⟨hConsisΓ', hΓΓ', hMaximalΓ'⟩⟩ := exists_maximal_consistent_theory hConsisΓ;
+  existsi ⟨Γ', (by aesop), (by aesop)⟩;
+  assumption;
+
+def CanonicalModel (Λ : AxiomSet β) : Model (MaximalConsistentTheory Λ) β where
   frame (Γ Δ) := ∀ (p : Formula β), (□p ∈ Γ.theory) → (p ∈ Δ.theory)
   val (Γ a) := (atom a) ∈ Γ.theory
 
 @[simp]
-lemma CanonicalModel_frame {Λ : Logic β} {MΓ MΔ : MaximalConsistentTheory Λ} :
-  (CanonicalModel Λ).frame MΓ MΔ ↔ (∀ (p : Formula β), (□p ∈ MΓ.theory) → (p ∈ MΔ.theory))
+lemma CanonicalModel_frame {Λ : AxiomSet β} {Ω MΔ : MaximalConsistentTheory Λ} :
+  (CanonicalModel Λ).frame Ω MΔ ↔ (∀ (p : Formula β), (□p ∈ Ω.theory) → (p ∈ MΔ.theory))
   := by rfl
 
 @[simp]
-lemma CanonicalModel_val {Λ : Logic β} {MΓ : MaximalConsistentTheory Λ} {a : β} :
-  a ∈ (CanonicalModel Λ).val MΓ ↔ (atom a) ∈ MΓ.theory
+lemma CanonicalModel_val {Λ : AxiomSet β} {Ω : MaximalConsistentTheory Λ} {a : β} :
+  a ∈ (CanonicalModel Λ).val Ω ↔ (atom a) ∈ Ω.theory
   := by rfl
 
-attribute [simp] Context.Models
-
-/-- a.k.a. _Truth Lemma_ -/
 lemma mem_maximalConsistentTheory_iff
-  {MΓ : MaximalConsistentTheory Λ} {p : Formula β} : (MΓ ⊧ᴹˢ[CanonicalModel Λ] p) ↔ (p ∈ MΓ.theory) := by
+  {Ω : MaximalConsistentTheory Λ} {p : Formula β} : (Ω ⊧ᴹˢ[CanonicalModel Λ] p) ↔ (p ∈ Ω.theory) := by
   induction p using rec' with
   | hatom a => simp;
-  | hfalsum => have := consistent_no_falsum MΓ.consistent; aesop;
+  | hfalsum => simpa [Satisfies.bot_def] using consistent_no_falsum' Ω.consistent;
   | himp p q ihp ihq =>
     simp [ihp, ihq];
-    sorry;
-  | hbox p ih =>
-    simp;
     constructor;
-    . sorry;
-    . sorry;
+    . intro h;
+      sorry;
+    . intro hpq hp;
+      sorry;
+  | hbox p ih =>
+    constructor;
+    . contrapose;
+      intro h;
+      sorry;
+    . intro h Δ h₂;
+      have b := h₂ _ h;
+      sorry;
+
 
 lemma mem_maximalConsistentTheory_iff'
-  {MΓ : MaximalConsistentTheory Λ} {Γ : Context β} : (MΓ ⊧ᴹˢ[CanonicalModel Λ] Γ) ↔ (Γ ⊆ MΓ.theory) := by
+  {Ω : MaximalConsistentTheory Λ} {Γ : Context β} : (Ω ⊧ᴹˢ[CanonicalModel Λ] Γ) ↔ (Γ ⊆ Ω.theory) := by
   simp [Set.subset_def];
   constructor;
   . intro h p hp; exact (mem_maximalConsistentTheory_iff).mp (h p hp);
   . intro h p hp; exact (mem_maximalConsistentTheory_iff).mpr (h p hp);
 
-theorem LogicK.Hilbert.completes : Completeness (MaximalConsistentTheory (𝐊 : Logic β)) (𝐊 : Logic β) := by
+theorem LogicK.Hilbert.completes : Completeness (𝐊 : AxiomSet β) (MaximalConsistentTheory (𝐊 : AxiomSet β)) := by
   apply intro_Completeness;
 
   intro Γ hConsisΓ;
-  let ⟨MΓ, hMΓ⟩ := lindenbaum' Γ hConsisΓ;
+  let ⟨Ω, hΩ⟩ := lindenbaum hConsisΓ;
 
   existsi (CanonicalModel 𝐊).frame;
   constructor;
   . apply LogicK.def_FrameClass;
-  . existsi (CanonicalModel 𝐊).val, MΓ;
-    apply mem_maximalConsistentTheory_iff'.mpr hMΓ;
+  . existsi (CanonicalModel 𝐊).val, Ω;
+    apply mem_maximalConsistentTheory_iff'.mpr hΩ;
 
-
-/-
-section
-
-variable {Λ : Logic β} {Γ : Context β} (consisΓ : Consistent Λ Γ)
-
-lemma exists_maximal_consistent_context (consisΓ : Consistent Λ Γ):
-  ∃ (Γ' : Context β), (Consistent Λ Γ' ∧ Γ ⊆ Γ' ∧ ∀ Δ, Consistent Λ Δ → Γ' ⊆ Δ → Δ = Γ') := sorry
-
-noncomputable def MaximalConsistentContext : Context β := Classical.choose $ exists_maximal_consistent_context consisΓ
-
-abbrev MCC := MaximalConsistentContext consisΓ
-
-lemma consistent_MCC : (MCC consisΓ).Consistent Λ := (Classical.choose_spec $ exists_maximal_consistent_context consisΓ).1
-
-lemma subset_MCC : Γ ⊆ (MCC consisΓ) := (Classical.choose_spec $ exists_maximal_consistent_context consisΓ).2.1
-
-lemma maximal_MCC : ∀ Δ, (Δ.Consistent Λ) → (MCC consisΓ) ⊆ Δ → Δ = (MCC consisΓ) := (Classical.choose_spec $ exists_maximal_consistent_context consisΓ).2.2
-
-end
--/
-
-/-
-section
-
-class ConsistentContext (Λ : Logic β) (Γ : Context β) where
-  consistent : Consistent Λ Γ
-
-class MaximalConsistentContext (Λ : Logic β) (Γ : Context β) extends ConsistentContext Λ Γ where
-  maximal : Maximal Γ
-
-abbrev CC (Λ : Logic β) := ConsistentContext Λ
-abbrev MCC (Λ : Logic β) := MaximalConsistentContext Λ
-
-end
-
-namespace ConsistentContext
-
-open ConsistentContext
-
-variable [CC Λ Γ]
-
-lemma no_falsum : ⊥ ∉ Γ := by
-  by_contra hC;
-  have h₁ : Γ ⊢ᴹ(Λ) ⊥ := axm hC;
-  have h₂ : IsEmpty (Γ ⊢ᴹ(Λ) ⊥) := by simpa [Consistent, Inconsistent] using consistent;
-  exact h₂.false h₁;
-
-end ConsistentContext
-
-
-namespace MaximalConsistentContext
-
-open MaximalConsistentContext
-
-variable [MCC Λ Γ]
-
-lemma closed_modus_ponens : (p ∈ Γ) → ((p ⟶ q) ∈ Γ) → (q ∈ Γ) := by
-  intro hp hpq; by_contra hnq;
-
-  have hp : Γ ⊢ᴹ(Λ) p := Deduction.axm hp;
-  have hpq : Γ ⊢ᴹ(Λ) (p ⟶ q) := Deduction.axm hpq;
-  have hq : Γ ⊢ᴹ(Λ) q := Deduction.modus_ponens hpq hp;
-
-  have hnq : Γ ⊢ᴹ(Λ) ~q := by {
-    sorry; -- have : ~q ∈ Γ; have b := maximal; sorry;
-    -- exact Deduction.axm this;
-  }
-  exact consistent ⟨hq⟩ ⟨hnq⟩;
-
-end MaximalConsistentContext
-
-end
-
-
-section Lemmas
-
-variable {Λ : Logic β}
-variable [Encodable β]
-
-lemma def_not_FrameclassSatisfiable {Γ : Context β} {p : Formula β} : ∀ {f : Frame α}, (Γ ⊭ᴹᶠ[f] p) ↔ (FrameSatisfiable f (insert (~p) Γ)) := by
-  simp_all [FrameclassSatisfiable, FrameSatisfiable, ModelSatisfiable];
-  aesop;
-
-lemma def_not_Consistent {Γ : Context β} {p : Formula β} : (Γ ⊬ᴹ(Λ)! p) ↔ ((insert (~p) Γ).Consistent Λ) := by
-  simp_all [Consistent, Inconsistent];
-  constructor;
-  . intro h;
-    by_contra hC; simp at hC;
-    have h₁ : insert (~p) Γ ⊢ᴹ(Λ) (p ⟶ ⊥) := by {
-      have : insert (~p) Γ ⊢ᴹ(Λ) ~p := Deduction.axm (by simp);
-      simpa [Formula.neg] using this;
-    };
-    sorry;
-  . intro h;
-    by_contra hC; simp at hC;
-    suffices (insert (~p) Γ ⊢ᴹ(Λ) ⊥) by have : (insert (~p) Γ ⊢ᴹ(Λ)! ⊥) := ⟨this⟩; aesop;
-    have h₁ : insert (~p) Γ ⊢ᴹ(Λ) p := Deduction.weakening' _ (by simp) hC.some;
-    have h₂ : insert (~p) Γ ⊢ᴹ(Λ) p ⟶ ⊥ := by {
-      have : insert (~p) Γ ⊢ᴹ(Λ) ~p := Deduction.axm (by simp);
-      simpa [Formula.neg_eq] using this;
-    };
-    exact Deduction.modus_ponens h₂ h₁;
-
-lemma intro_Completeness : (∀ (f : Frame α) (Γ : Context β), Γ.FrameSatisfiable f) → (Completeness α Λ)  := by
-  simp only [Completeness];
-  intro h f Γ p _ hΓp;
-  have h₁ : Γ ⊭ᴹᶠ[f] p := (def_not_FrameclassSatisfiable.mpr $ h f (insert (~p) Γ));
-  have := h₁ hΓp;
-  contradiction;
-
-section LindenbaumAux
-
-variable (Λ : Logic β) [∀ Γ p, Decidable (Consistent Λ (insert p Γ))] [Encodable α]
-
-def lindenbaum_next (p : Formula β) (Γ : CC Λ) : CC Λ :=
-  if h : (insert p Γ.ctx).Consistent Λ then ⟨(insert p Γ.ctx), by assumption;⟩
-  else ⟨
-    insert (~p) Γ.ctx,
-    by
-      by_contra hC; sorry;
-      -- simp [def_not_Consistent] at h;
-  ⟩
-
-def lindenbaum_family (Γ : CC Λ) : ℕ → (CC Λ)
-  | 0     => Γ
-  | n + 1 =>
-    match (Formula.decode n) with
-    | none   => lindenbaum_family Γ n
-    | some p => lindenbaum_next Λ p (lindenbaum_family Γ n)
-
-notation Γ "[" Λ "," i "]" => lindenbaum_family Λ Γ i
-
-lemma lindenbaum_subset (Γ : CC Λ) (n : ℕ) : (Γ[Λ, n]).ctx ⊆ (Γ[Λ, n + 1]).ctx := by
-  simp [lindenbaum_family, lindenbaum_next];
-  aesop;
-
-lemma maximal (Γ : CC Λ) (p : Formula β) : (p ∈ Γ[Λ, p.encode + 1].ctx) ∨ (p ∉ Γ[Λ, p.encode + 1].ctx) := by
-  induction Formula.encode p with
-  | zero =>
-    simp [lindenbaum_family, lindenbaum_next, Formula.decode, (show ¬Consistent Λ (insert ⊥ Γ.ctx) by have := Inconsistent.no_falsum_include Λ Γ.ctx; aesop)];
-    sorry;
-  | succ n ih =>
-    sorry;
-
-end LindenbaumAux
-
-lemma lindenbaum (Γ : CC Λ) : ∃ (Γ' : MCC Λ), Γ.ctx ⊆ Γ'.ctx := by sorry;
-
-def CanonicalModel (Λ : Logic β) : Model (MCC Λ) β where
-  rel (Γ Δ) := ∀ (p : Formula β), (□p ∈ Γ.ctx) → (p ∈ Δ.ctx)
-  val (Γ a) := (atom a) ∈ Γ.ctx
-
-lemma TruthLemma (mΓ : MCC Λ) (p : Formula β) : (mΓ.ctx ⊨ᴹᵐ[CanonicalModel Λ] p) ↔ (p ∈ mΓ.ctx) := by
-  induction p using rec' with
-  | hatom a => sorry;
-  | hfalsum =>
-    constructor;
-    . intro h; sorry;
-    . intro h; have := ConsistentContext.no_falsum mΓ.toConsistentContext h; contradiction;
-  | himp p q ihp ihq =>
-    constructor;
-    . intro h; sorry;
-    . intro h; sorry;
-  | hbox p ih => sorry;
-
-lemma TruthLemma' (mΓ : MCC Λ) (Δ : CC Λ) : (mΓ.ctx ⊨ᴹᵐ[CanonicalModel Λ] Δ.ctx) ↔ (Δ.ctx ⊆ mΓ.ctx) := by
-  simp [Context.ModelConsequence];
-  constructor;
-  . intro h p hp; exact (TruthLemma mΓ p).mp $ h p hp;
-  . intro h p hp;
-    have ⟨mΔ, hmΔ⟩ := lindenbaum Δ;
-    have h₁ := (TruthLemma mΔ p).mpr $ Set.mem_of_subset_of_mem hmΔ hp;
-    intros;
-    sorry;
-
--- lemma model_existence (Γ : Context β) : Γ.consistent Λ ↔ (frameclass_satisfiable (FrameClass.Trivial α) Γ) := by sorry;
-
-lemma tmp1 (p : Formula β) : mΓ ⊧ᴹˢ[CanonicalModel Λ] p := by
-  sorry
-
-lemma canonical_satisfiable {Γ : CC Λ} {mΓ : MCC Λ} (h : mΓ.ctx ⊨ᴹᵐ[CanonicalModel Λ] Γ.ctx) : (FrameSatisfiable (CanonicalModel Λ).toFrame Γ.ctx) := by
-  simp [FrameSatisfiable];
-  existsi (CanonicalModel Λ).val;
-  simp [ModelSatisfiable];
-  existsi mΓ;
-  intro p hp;
-  have b := (TruthLemma' mΓ Γ).mp h;
-
-end Lemmas
-
-/-
-namespace CanonicalModel
-
-variable (Λ : Set (Formula β))
-
-lemma isReflexive (_ : Λ ⊆ 𝐓) : (@CanonicalModel β Λ).toFrame.Reflexive := by sorry;
-
-lemma isSymmetric (_ : Λ ⊆ 𝐁): (@CanonicalModel β Λ).toFrame.Symmetric := by sorry;
-
-lemma isSerial (_ : Λ ⊆ 𝐃): (@CanonicalModel β Λ).toFrame.Serial := by sorry;
-
-lemma isTransitive (_ : Λ ⊆ 𝟒): (@CanonicalModel β Λ).toFrame.Transitive := by sorry;
-
-lemma isEuclidean (_ : Λ ⊆ 𝟓): (@CanonicalModel β Λ).toFrame.Euclidean := by sorry;
-
-end CanonicalModel
--/
-
-theorem Hilbert.LogicK.completeness : Completeness (MCC (𝐊 : Logic β)) (𝐊 : Logic β) := by
-  apply intro_Completeness;
-  intro f Γ;
-  simp [FrameSatisfiable];
-  existsi (CanonicalModel 𝐊).val;
-  simp [ModelSatisfiable];
-
-  wlog hC : (Γ.Consistent 𝐊) with H; {
-    simp only [Consistent, Inconsistent, not_nonempty_iff, not_isEmpty_iff] at hC;
-    have b := LogicK.Hilbert.sounds (CanonicalModel 𝐊).toFrame;
-  }
-
-  let ⟨mΓ, hmΓ⟩ := lindenbaum ⟨Γ, hC⟩;
-  have h := (TruthLemma' mΓ ⟨Γ, hC⟩).mpr hmΓ;
-
-  apply canonical_satisfiable h;
-  trivial;
--/
 end LO.Modal.Normal
